coq/proof/Inject.v
@@ -1,0 +1,49 @@
+Require Import syntax.
+Require Import alist.
+Require Import FMapWeakList.
+
+Require Import Classical.
+Require Import Coqlib.
+Require Import infrastructure.
+Require Import Metatheory.
+Import LLVMsyntax.
+Import LLVMinfra.
+Require Import opsem.
+
+Require Import sflib.
+Require Import paco.
+Import Opsem.
+
+Require Import TODO.
+Require Import GenericValues.
+Require Import Nop.
+Require Import SimulationLocal.
+Require InvMem.
+Require InvState.
+
+(* TODO: name *)
+Definition inject_locals
+           (inv:InvMem.Rel.t)
+           (locals_src locals_tgt:GVsMap): Prop :=
+  forall (i:id) (gv_src:GenericValue) (LU_SRC: lookupAL _ locals_src i = Some gv_src),
+  exists gv_tgt,
+    <<LU_TGT: lookupAL _ locals_tgt i = Some gv_tgt>> /\
+    <<INJECT: genericvalues_inject.gv_inject inv.(InvMem.Rel.inject) gv_src gv_tgt>>.
+
+Definition inject_allocas
+           (inv:InvMem.Rel.t)
+           (alc_src alc_tgt:list mblock): Prop :=
+  list_forall2
+    (fun a_src a_tgt => inv.(InvMem.Rel.inject) a_src = Some (a_tgt, 0))
+    alc_src alc_tgt.
+
+Definition CONF_TODO: Prop. Admitted.
+
+Lemma targetdata_dec
+      (TD_src TD_tgt:TargetData):
+  {TD_src = TD_tgt} + {TD_src <> TD_tgt}.
+Proof.
+  decide equality.
+  - apply namedts_dec.
+  - apply layouts_dec.
+Qed.
