coq/proof/SimulationVali.v
@@ -1,0 +1,341 @@
+Require Import syntax.
+Require Import alist.
+Require Import FMapWeakList.
+
+Require Import Classical.
+Require Import Coqlib.
+Require Import infrastructure.
+Require Import Metatheory.
+Import LLVMsyntax.
+Import LLVMinfra.
+Require Import opsem.
+
+Require Import sflib.
+Require Import paco.
+Import Opsem.
+
+Require Import TODO.
+Require Import Validator.
+Require Import GenericValues.
+Require Import SimulationLocal.
+Require InvMem.
+Require InvState.
+
+
+Set Implicit Arguments.
+
+
+Definition CONF_TODO: Prop. Admitted.
+
+(* TODO: position *)
+Definition get_blocks (f:fdef): blocks :=
+  let '(fdef_intro _ blocks) := f in
+  blocks.
+
+Inductive vali_state_sim
+          (conf_src conf_tgt:Config)
+          (stack0_src stack0_tgt:ECStack)
+          (invmem:InvMem.Rel.t)
+          (idx:nat)
+          (st_src st_tgt:State): Prop :=
+| vali_state_sim_intro
+    m_src m_tgt
+    fdef_hint cmds_hint
+    inv inv_term
+    invst
+    (CONF: CONF_TODO) (* m_src, m_tgt, conf_src, conf_tgt *)
+    (ECS_SRC: st_src.(ECS) = stack0_src)
+    (ECS_TGT: st_tgt.(ECS) = stack0_tgt)
+    (FDEF: valid_fdef m_src m_tgt st_src.(EC).(CurFunction) st_tgt.(EC).(CurFunction) fdef_hint)
+    (CMDS: valid_cmds m_src m_tgt st_src.(EC).(CurCmds) st_tgt.(EC).(CurCmds) cmds_hint inv = Some inv_term)
+    (TERM: valid_terminator fdef_hint inv_term m_src m_tgt
+                            st_src.(EC).(CurFunction).(get_blocks)
+                            st_tgt.(EC).(CurFunction).(get_blocks)
+                            st_src.(EC).(CurBB).(fst)
+                            st_src.(EC).(Terminator)
+                            st_tgt.(EC).(Terminator))
+    (STATE: InvState.Rel.sem conf_src conf_tgt st_src st_tgt invst invmem inv)
+    (MEM: InvMem.Rel.sem conf_src conf_tgt st_src.(Mem) st_tgt.(Mem) invmem)
+.
+
+Lemma vali_init
+      m_src m_tgt
+      conf_src conf_tgt
+      stack0_src stack0_tgt
+      fdef_src fdef_tgt
+      fdef_hint
+      args_src args_tgt
+      mem_src mem_tgt
+      inv
+      ec_src
+      (FDEF: valid_fdef m_src m_tgt fdef_src fdef_tgt fdef_hint)
+      (ARGS: list_forall2 (genericvalues_inject.gv_inject inv.(InvMem.Rel.inject)) args_src args_tgt)
+      (MEM: InvMem.Rel.sem conf_src conf_tgt mem_src mem_tgt inv)
+      (CONF: CONF_TODO)
+      (INIT: init_fdef conf_src fdef_src args_src ec_src):
+  exists ec_tgt idx,
+    init_fdef conf_tgt fdef_tgt args_tgt ec_tgt /\
+    vali_state_sim
+      conf_src conf_tgt
+      stack0_src stack0_tgt
+      inv idx
+      (mkState ec_src stack0_src mem_src)
+      (mkState ec_tgt stack0_tgt mem_tgt).
+Proof.
+Admitted.
+
+(* TODO: position *)
+Ltac condtac :=
+  repeat
+    (try match goal with
+         | [H: ?a = ?a |- _] => clear H
+         | [H: context[match ?c with
+                       | [] => _
+                       | _::_ => _
+                       end] |- _] =>
+           let COND := fresh "COND" in
+           destruct c eqn:COND
+         | [H: context[match ?c with
+                       | Some _ => _
+                       | None => _
+                       end] |- _] =>
+           let COND := fresh "COND" in
+           destruct c eqn:COND
+         | [H: context[if ?c then _ else _] |- _] =>
+           let COND := fresh "COND" in
+           destruct c eqn:COND
+         | [H: Some _ = Some _ |- _] => inv H
+         | [H: context[let (_, _) := ?p in _] |- _] => destruct p
+         | [H: negb _ = false |- _] =>
+           apply negb_false_iff in H
+         | [H: proj_sumbool (typ_dec ?a ?b) = true |- _] =>
+           destruct (typ_dec a b)
+         | [H: proj_sumbool (l_dec ?a ?b) = true |- _] =>
+           destruct (l_dec a b)
+         end;
+     unfold Debug.debug_print_validation_process in *;
+     subst; ss).
+
+(* TODO: position *)
+Lemma has_false_False
+      conf_src conf_tgt st_src st_tgt invst invmem inv
+      (HAS_FALSE: Hints.Invariant.has_false inv)
+      (SEM: InvState.Rel.sem conf_src conf_tgt st_src st_tgt invst invmem inv):
+  False.
+Proof.
+Admitted.
+
+(* TODO: position *)
+Lemma postcond_cmd_sound
+      conf_src st0_src cmd_src cmds_src
+      conf_tgt st0_tgt cmd_tgt cmds_tgt
+      invst0 invmem0 inv0
+      st1_tgt evt inv1
+      (CMDS_SRC: st0_src.(EC).(CurCmds) = cmd_src :: cmds_src)
+      (CMDS_TGT: st0_tgt.(EC).(CurCmds) = cmd_tgt :: cmds_tgt)
+      (POSTCOND: Postcond.postcond_cmd cmd_src cmd_tgt inv0 = Some inv1)
+      (STATE: InvState.Rel.sem conf_src conf_tgt st0_src st0_tgt invst0 invmem0 inv0)
+      (MEM: InvMem.Rel.sem conf_src conf_tgt st0_src.(Mem) st0_tgt.(Mem) invmem0)
+      (STEP_TGT: sInsn conf_tgt st0_tgt st1_tgt evt):
+  exists st1_src invst1 invmem1,
+    <<STEP_SRC: sInsn conf_src st0_src st1_src evt>> /\
+    <<STATE: InvState.Rel.sem conf_src conf_tgt st1_src st1_tgt invst1 invmem1 inv1>>/\
+    <<MEM: InvMem.Rel.sem conf_src conf_tgt st1_src.(Mem) st1_tgt.(Mem) invmem1>> /\
+    <<MEMLE: InvMem.Rel.le invmem0 invmem1>>.
+Proof.
+Admitted.
+
+(* TODO: position *)
+Lemma apply_infrule_sound
+      m_src m_tgt
+      conf_src st_src
+      conf_tgt st_tgt
+      invst0 invmem0 inv0
+      infrule
+      (CONF: CONF_TODO) (* m_src, m_tgt, conf_src, conf_tgt *)
+      (STATE: InvState.Rel.sem conf_src conf_tgt st_src st_tgt invst0 invmem0 inv0)
+      (MEM: InvMem.Rel.sem conf_src conf_tgt st_src.(Mem) st_tgt.(Mem) invmem0):
+  exists invst1 invmem1,
+    <<STATE: InvState.Rel.sem conf_src conf_tgt st_src st_tgt invst1 invmem1
+                              (Infrules.apply_infrule m_src m_tgt infrule inv0)>> /\
+    <<MEM: InvMem.Rel.sem conf_src conf_tgt st_src.(Mem) st_tgt.(Mem) invmem1>> /\
+    <<MEMLE: InvMem.Rel.le invmem0 invmem1>>.
+Proof.
+Admitted.
+
+(* TODO: position *)
+Lemma apply_infrules_sound
+      m_src m_tgt
+      conf_src st_src
+      conf_tgt st_tgt
+      invst0 invmem0 inv0
+      infrules
+      (CONF: CONF_TODO) (* m_src, m_tgt, conf_src, conf_tgt *)
+      (STATE: InvState.Rel.sem conf_src conf_tgt st_src st_tgt invst0 invmem0 inv0)
+      (MEM: InvMem.Rel.sem conf_src conf_tgt st_src.(Mem) st_tgt.(Mem) invmem0):
+  exists invst1 invmem1,
+    <<STATE: InvState.Rel.sem conf_src conf_tgt st_src st_tgt invst1 invmem1
+                              (Infrules.apply_infrules m_src m_tgt infrules inv0)>> /\
+    <<MEM: InvMem.Rel.sem conf_src conf_tgt st_src.(Mem) st_tgt.(Mem) invmem1>> /\
+    <<MEMLE: InvMem.Rel.le invmem0 invmem1>>.
+Proof.
+  unfold Infrules.apply_infrules. rewrite <- fold_left_rev_right.
+  move infrules at top. revert_until infrules. induction (rev infrules); i.
+  - esplits; eauto.
+    admit. (* InvMem.Rel.le refl *)
+  - exploit IHl0; eauto. i. des.
+    exploit apply_infrule_sound; eauto. i. des.
+    esplits; eauto.
+    + ss. eauto.
+    + admit. (* InvMem.Rel.le trans *)
+Admitted.
+
+(* TODO: position *)
+Lemma reduce_maydiff_sound
+      conf_src st_src
+      conf_tgt st_tgt
+      invst invmem inv
+      (CONF: CONF_TODO) (* m_src, m_tgt, conf_src, conf_tgt *)
+      (STATE: InvState.Rel.sem conf_src conf_tgt st_src st_tgt invst invmem inv)
+      (MEM: InvMem.Rel.sem conf_src conf_tgt st_src.(Mem) st_tgt.(Mem) invmem):
+  <<STATE: InvState.Rel.sem conf_src conf_tgt st_src st_tgt invst invmem
+                            (Postcond.reduce_maydiff inv)>> /\
+  <<MEM: InvMem.Rel.sem conf_src conf_tgt st_src.(Mem) st_tgt.(Mem) invmem>>.
+Proof.
+Admitted.
+
+(* TODO: position *)
+Lemma implies_sound
+      conf_src st_src
+      conf_tgt st_tgt
+      invst invmem inv0 inv1
+      (CONF: CONF_TODO) (* m_src, m_tgt, conf_src, conf_tgt *)
+      (IMPLIES: Hints.Invariant.implies inv0 inv1)
+      (STATE: InvState.Rel.sem conf_src conf_tgt st_src st_tgt invst invmem inv0)
+      (MEM: InvMem.Rel.sem conf_src conf_tgt st_src.(Mem) st_tgt.(Mem) invmem):
+  <<STATE: InvState.Rel.sem conf_src conf_tgt st_src st_tgt invst invmem inv1>> /\
+  <<MEM: InvMem.Rel.sem conf_src conf_tgt st_src.(Mem) st_tgt.(Mem) invmem>>.
+Proof.
+Admitted.
+
+(* TODO: position *)
+Lemma inject_value_sound
+      conf_src st_src val_src
+      conf_tgt st_tgt val_tgt
+      invst invmem inv
+      gval_src
+      (STATE: InvState.Rel.sem conf_src conf_tgt st_src st_tgt invst invmem inv)
+      (MEM: InvMem.Rel.sem conf_src conf_tgt st_src.(Mem) st_tgt.(Mem) invmem)
+      (INJECT: Hints.Invariant.inject_value inv val_src val_tgt)
+      (VAL_SRC: InvState.Unary.sem_valueT conf_src st_src invst.(InvState.Rel.src) val_src = Some gval_src):
+  exists gval_tgt,
+    <<VAL_TGT: InvState.Unary.sem_valueT conf_tgt st_tgt invst.(InvState.Rel.tgt) val_tgt = Some gval_tgt>> /\
+    <<INJECT: genericvalues_inject.gv_inject invmem.(InvMem.Rel.inject) gval_src gval_tgt>>.
+Proof.
+Admitted.
+
+(* TODO: position *)
+Lemma sem_valueT_physical
+      conf st inv val:
+  InvState.Unary.sem_valueT conf st inv (Exprs.ValueT.lift Exprs.Tag.physical val) =
+  getOperandValue conf.(CurTargetData) val st.(EC).(Locals) conf.(Globals).
+Proof. destruct val; ss. Qed.
+
+Lemma vali_sim
+      conf_src conf_tgt
+      (CONF: CONF_TODO):
+  (vali_state_sim conf_src conf_tgt) <6= (sim_local conf_src conf_tgt).
+Proof.
+  intros stack0_src stack0_tgt.
+  pcofix CIH.
+  intros inv0 idx0 st_src st_tgt SIM. pfold.
+  generalize (classic (stuck_state conf_src st_src)). intro STUCK_SRC. des.
+  { destruct (s_isFinialState conf_src st_src) eqn:FINAL_SRc; cycle 1.
+    - (* error *)
+      eapply _sim_local_error; eauto. econs; eauto.
+    - (* final *)
+      admit.
+  }
+  destruct st_src, st_tgt. destruct EC0, EC1.
+  inv SIM. ss.
+  destruct CurCmds0; condtac;
+    (try by exfalso; eapply has_false_False; eauto).
+  - (* term *)
+    unfold valid_terminator in TERM.
+    condtac;
+      (try by exfalso; eapply has_false_False; eauto).
+    apply NNPP in STUCK_SRC. des.
+    inv STUCK_SRC; destruct Terminator1; condtac.
+    (* TODO: switch case *)
+    + (* return *)
+      unfold returnUpdateLocals in *. condtac.
+      exploit inject_value_sound; eauto.
+      { rewrite sem_valueT_physical. eauto. }
+      rewrite sem_valueT_physical. s. i. des.
+      eapply _sim_local_return; eauto; ss.
+    + (* return_void *)
+      eapply _sim_local_return_void; eauto; ss.
+    + (* br *)
+      exploit inject_value_sound; eauto.
+      { rewrite sem_valueT_physical. eauto. }
+      rewrite sem_valueT_physical. s. i. des.
+      eapply _sim_local_step.
+      { admit. (* tgt not stuck *) }
+      i. inv STEP. ss.
+      esplits; eauto.
+      { econs 1. econs; eauto. rewrite COND5. eauto. }
+      { admit. (* InvMem.Rel.le refl *) }
+      right. apply CIH.
+      instantiate (1 := mkState _ _ _). econs; eauto; ss.
+      * admit. (* valid_fdef *)
+      * admit. (* valid_cmds *)
+      * admit. (* valid_terminator *)
+      * admit. (* InvState.Rel.sem *)
+    + (* br, bogus: see https://github.com/snu-sf/llvmberry/issues/310 *)
+      admit.
+    + (* br_uncond *)
+      eapply _sim_local_step.
+      { admit. (* tgt not stuck *) }
+      i. inv STEP. ss.
+      esplits; eauto.
+      { econs 1. econs; eauto. }
+      { admit. (* InvMem.Rel.le refl *) }
+      right. apply CIH.
+      instantiate (1 := mkState _ _ _). econs; eauto; ss.
+      * admit. (* valid_fdef *)
+      * admit. (* valid_cmds *)
+      * admit. (* valid_terminator *)
+      * admit. (* InvState.Rel.sem *)
+  - (* cmd *)
+    eapply _sim_local_step.
+    { (* tgt not stuck *)
+      admit.
+    }
+    i.
+    (* TODO: call is ignored! *)
+    exploit postcond_cmd_sound; eauto; ss. i. des.
+    exploit apply_infrules_sound; eauto; ss. i. des.
+    exploit reduce_maydiff_sound; eauto; ss. i. des.
+    exploit implies_sound; eauto; ss. i. des.
+    esplits; eauto.
+    + econs 1. eauto.
+    + right. apply CIH. econs; eauto.
+      * admit. (* valid_fdef *)
+      * admit. (* valid_cmds *)
+      * admit. (* valid_terminator *)
+Admitted.
+
+Lemma vali_sim_func
+      m_src m_tgt
+      conf_src conf_tgt
+      fdef_src fdef_tgt
+      fdef_hint
+      (CONF: CONF_TODO)
+      (FDEF: valid_fdef m_src m_tgt fdef_src fdef_tgt fdef_hint):
+  sim_func conf_src conf_tgt fdef_src fdef_tgt.
+Proof.
+  ii.
+  exploit vali_init; eauto. i. des.
+  esplits; eauto.
+  apply vali_sim; eauto.
+Qed.
